Weakening + universe ended without much trouble. Completeness in Neutral.v is not true anymore, however.

theories/LogicalRelation/Neutral.v
@@ -1,5 +1,5 @@
 From LogRel.AutoSubst Require Import core unscoped Ast Extra.
-From LogRel Require Import Utils BasicAst Notations Context NormalForms UntypedReduction Weakening GenericTyping LogicalRelation DeclarativeInstance.
+From LogRel Require Import Utils BasicAst Notations LContexts Context NormalForms UntypedReduction Weakening GenericTyping LogicalRelation DeclarativeInstance.
 From LogRel.LogicalRelation Require Import Induction Reflexivity Irrelevance Escape.
 
 Set Universe Polymorphism.
@@ -7,43 +7,47 @@ Set Universe Polymorphism.
 Section Neutral.
 Context `{GenericTypingProperties}.
 
-Definition neu {l Γ A} : Ne[Γ |- A] -> [Γ |- A] -> [ Γ |- A ~ A : U] -> [Γ ||-<l> A].
+Definition neu {l wl Γ A} : Ne[Γ |- A]< wl > -> [Γ |- A]< wl > -> [ Γ |- A ~ A : U]< wl > -> [Γ ||-<l> A]< wl >.
 Proof.
   intros neA wtyA reflA. apply LRne_.
   exists A; [gen_typing|..]; assumption.
 Defined.
 
-Lemma neU {l Γ A n} (h : [Γ ||-U<l> A]) :
-  Ne[Γ |- n : A] ->
-  [Γ |- n : A] ->
-  [Γ |- n ~ n : A] ->
-  [LogRelRec l | Γ ||-U n : A | h].
+Lemma neU {l wl Γ A n} (h : [Γ ||-U<l> A]< wl >) :
+  Ne[Γ |- n : A]< wl > ->
+  [Γ |- n : A]< wl > ->
+  [Γ |- n ~ n : A]< wl > ->
+  [LogRelRec l | Γ ||-U n : A | h]< wl >.
 Proof.
-  assert [Γ |- A ≅ U] by (destruct h; gen_typing).
+  assert [Γ |- A ≅ U]< wl > by (destruct h; gen_typing).
   intros; exists n.
   * eapply redtmwf_conv; tea; now eapply redtmwf_refl.
   * now eapply NeType, tm_ne_whne.
-  * eapply tm_nf_conv; [|gen_typing|eassumption].
-    now eapply tm_ne_nf.
+  * eapply tm_nf_conv.
+    -- now eapply tm_ne_nf.
+    -- assumption.
   * eapply convtm_conv; tea; gen_typing.
   * eapply RedTyRecBwd, neu. 2,3: gen_typing.
     eapply ty_ne_term, tm_ne_conv; now gen_typing.
 Defined.
 
 
-Lemma neElim {Γ l K} : [Γ ||-<l> K] -> whne K -> [Γ ||-ne K].
+Lemma neElim {wl Γ l K} : [Γ ||-<l> K]< wl > -> whne wl K -> [Γ ||-ne K]< wl >.
 Proof.
-  intros h; pattern l,Γ,K,h; eapply LR_rect_TyUr;
-  clear l Γ K h.
-  - intros ??? [??? r] ne; pose proof (redtywf_whne r  ne); subst; inversion ne.
+  intros h; pattern l,wl,Γ,K,h; eapply LR_rect_TyUr;
+  clear l wl Γ K h.
+  - intros ???? [??? r] ne; pose proof (redtywf_whne r  ne); subst; inversion ne.
   - intros; assumption.
-  - intros ??? [?? red] ?? ne ; cbn in *.
+  - intros ???? [?? red] ?? ne ; cbn in *.
     rewrite (redtywf_whne red ne) in ne.
     inversion ne.
-  - intros ??? [red] ne.
+  - intros ???? [red] ne.
     rewrite (redtywf_whne red ne) in ne.
     inversion ne.
-  - intros ??? [red] ne.
+  - intros ???? [red] ne.
+    rewrite (redtywf_whne red ne) in ne.
+    inversion ne.
+  - intros ???? [red] ne.
     rewrite (redtywf_whne red ne) in ne.
     inversion ne.
 Qed.
@@ -51,11 +55,11 @@ Qed.
 Set Printing Primitive Projection Parameters.
 
 
-Lemma neuEq {l Γ A B} (RA : [Γ ||-<l> A]) :
-  Ne[Γ |- A] -> Ne[Γ |- B] ->
-  [Γ |- A] -> [Γ |- B] ->
-  [Γ |- A ~ B : U] ->
-  [Γ ||-<l> A ≅ B | RA].
+Lemma neuEq {l wl Γ A B} (RA : [Γ ||-<l> A]< wl >) :
+  Ne[Γ |- A]< wl > -> Ne[Γ |- B]< wl > ->
+  [Γ |- A]< wl > -> [Γ |- B]< wl > ->
+  [Γ |- A ~ B : U]< wl > ->
+  [Γ ||-<l> A ≅ B | RA]< wl >.
 Proof.
   intros neA neB wtyA wtyB eqAB.
   unshelve irrelevance0. 1: assumption. 3: reflexivity.
@@ -65,8 +69,8 @@ Proof.
   all: cbn; assumption.
 Qed.
 
-Lemma ty_app_ren {Γ Δ A f a dom cod} (ρ : Δ ≤ Γ) :
-  [Γ |- f : A] -> [Γ |- A ≅ tProd dom cod] -> [Δ |- a : dom⟨ρ⟩] -> [Δ |- tApp f⟨ρ⟩ a : cod[a .: ρ >> tRel]].
+Lemma ty_app_ren {wl Γ Δ A f a dom cod} (ρ : Δ ≤ Γ) :
+  [Γ |- f : A]< wl > -> [Γ |- A ≅ tProd dom cod]< wl > -> [Δ |- a : dom⟨ρ⟩]< wl > -> [Δ |- tApp f⟨ρ⟩ a : cod[a .: ρ >> tRel]]< wl >.
 Proof.
   intros.
   replace (cod[a .: ρ >> tRel]) with (cod⟨wk_up dom ρ⟩[a..]) by (now bsimpl).
@@ -75,11 +79,11 @@ Proof.
   gen_typing.
 Qed.
 
-Lemma convneu_app_ren {Γ Δ A f g a b dom cod} (ρ : Δ ≤ Γ) :
-  [Γ |- f ~ g : A] ->
-  [Γ |- A ≅ tProd dom cod] ->
-  [Δ |- a ≅ b : dom⟨ρ⟩] ->
-  [Δ |- tApp f⟨ρ⟩ a ~ tApp g⟨ρ⟩ b : cod[a .: ρ >> tRel]].
+Lemma convneu_app_ren {wl Γ Δ A f g a b dom cod} (ρ : Δ ≤ Γ) :
+  [Γ |- f ~ g : A]< wl > ->
+  [Γ |- A ≅ tProd dom cod]< wl > ->
+  [Δ |- a ≅ b : dom⟨ρ⟩]< wl > ->
+  [Δ |- tApp f⟨ρ⟩ a ~ tApp g⟨ρ⟩ b : cod[a .: ρ >> tRel]]< wl >.
 Proof.
   intros.
   replace (cod[a .: ρ >> tRel]) with (cod⟨wk_up dom ρ⟩[a..]) by (now bsimpl).
@@ -88,64 +92,63 @@ Proof.
   gen_typing.
 Qed.
 
-Lemma neu_app_ren {Γ Δ A n a dom cod} (ρ : Δ ≤ Γ) :
-  [|- Δ] ->
-  [Γ |- tProd dom cod] ->
-  Ne[Γ |- n : A] -> [Γ |- A ≅ tProd dom cod] -> Nf[Δ |- a : dom⟨ρ⟩] -> Ne[Δ |- tApp n⟨ρ⟩ a : cod[a .: ρ >> tRel]].
+Lemma neu_app_ren {wl Γ Δ A n a dom cod} (ρ : Δ ≤ Γ) :
+  [|- Δ]< wl > ->
+  [Γ |- tProd dom cod]< wl > ->
+  Ne[Γ |- n : A]< wl > -> [Γ |- A ≅ tProd dom cod]< wl > -> Nf[Δ |- a : dom⟨ρ⟩]< wl > -> Ne[Δ |- tApp n⟨ρ⟩ a : cod[a .: ρ >> tRel]]< wl >.
 Proof.
   intros.
   replace (cod[a .: ρ >> tRel]) with (cod⟨wk_up dom ρ⟩[a..]) by (now bsimpl).
   eapply tm_ne_app; [|eassumption].
-  change (Ne[Δ |- n⟨ρ⟩ : (tProd dom cod)⟨ρ⟩]).
-  eapply tm_ne_conv; [| |now eapply convty_wk].
+  change (Ne[Δ |- n⟨ρ⟩ : (tProd dom cod)⟨ρ⟩]< wl >).
+  eapply tm_ne_conv.
   + now eapply tm_ne_wk.
-  + now eapply wft_wk.
+  + now eapply convty_wk.
 Qed.
 
-Record complete {l Γ A} (RA : [Γ ||-<l> A]) := {
-  reifyTyConv : forall B, [Γ ||-<l> A ≅ B | RA] -> Nf[Γ |- B];
+Record complete {l wl Γ A} (RA : [Γ ||-<l> A]< wl >) := {
+  reifyTyConv : forall B, [Γ ||-<l> A ≅ B | RA]< wl > -> Nf[Γ |- B]< wl >;
   reflect : forall n n',
-    Ne[Γ |- n : A] ->
-    Ne[Γ |- n' : A] ->
-    [Γ |- n : A] ->
-    [Γ |- n' : A] ->
-    [Γ |- n ~ n' : A] ->
-    [Γ ||-<l> n : A | RA] × [Γ ||-<l> n ≅ n' : A| RA];
-  reify : forall a, [Γ ||-<l> a : A | RA] -> Nf[ Γ |- a : A];
+    Ne[Γ |- n : A]< wl > ->
+    Ne[Γ |- n' : A]< wl > ->
+    [Γ |- n : A]< wl > ->
+    [Γ |- n' : A]< wl > ->
+    [Γ |- n ~ n' : A]< wl > ->
+    [Γ ||-<l> n : A | RA]< wl > × [Γ ||-<l> n ≅ n' : A| RA]< wl >;
+  reify : forall a, [Γ ||-<l> a : A | RA]< wl > -> Nf[ Γ |- a : A]< wl >;
 }.
 
-Lemma complete_reflect_simpl {l Γ A} (RA : [Γ ||-<l> A]) (c : complete RA) :
-  forall n, Ne[Γ |- n : A] -> [Γ |- n : A] -> [Γ |- n ~ n : A] -> [Γ ||-<l> n : A | RA].
+Lemma complete_reflect_simpl {l wl Γ A} (RA : [Γ ||-<l> A]< wl >) (c : complete RA) :
+  forall n, Ne[Γ |- n : A]< wl > -> [Γ |- n : A]< wl > -> [Γ |- n ~ n : A]< wl > -> [Γ ||-<l> n : A | RA]< wl >.
 Proof.
 intros; eapply c.
 5: eassumption.
 all: assumption.
 Qed.
 
-Lemma complete_var0 {l Γ A A'} (RA : [Γ ,, A ||-<l> A']) :
+Lemma complete_var0 {l wl Γ A A'} (RA : [Γ ,, A ||-<l> A']< wl >) :
   complete RA ->
-  [Γ ,, A |- A⟨↑⟩ ≅ A'] ->
-  [Γ |- A] ->
-  [Γ ,, A ||-<l> tRel 0 : A' | RA].
+  [Γ ,, A |- A⟨↑⟩ ≅ A']< wl > ->
+  [Γ |- A]< wl > ->
+  [Γ ,, A ||-<l> tRel 0 : A' | RA]< wl >.
 Proof.
   intros cRA conv HA.
-  assert [Γ ,, A |- tRel 0 : A']
+  assert [Γ ,, A |- tRel 0 : A']< wl >
   by (eapply ty_conv; tea; escape; eapply (ty_var (wfc_wft EscRA) (in_here _ _))).
   eapply complete_reflect_simpl; tea.
   - eapply tm_ne_conv; tea. 
-    2: now escape. 
     now eapply tm_ne_rel.
   - eapply convneu_var; tea.
 Qed.
 
 
-Lemma complete_U : forall l Γ A (RA : [Γ ||-U< l > A]), complete (LRU_ RA).
+Lemma complete_U : forall l wl Γ A (RA : [Γ ||-U< l > A]< wl >), complete (LRU_ RA).
 Proof.
-intros l Γ A h0; split.
+intros l wl Γ A h0; split.
 - intros ? [].
   eapply ty_nf_red, ty_nf_sort; gen_typing.
 - intros ?? ???? h; pose proof (lrefl h); pose proof (urefl h).
-  assert [Γ |- A ≅ U] by (destruct h0; gen_typing); split.
+  assert [Γ |- A ≅ U]< wl > by (destruct h0; gen_typing); split.
   2: unshelve econstructor.
   1-3: now apply neU.
   + eapply RedTyRecBwd, neu. 2,3: try gen_typing.
@@ -156,20 +159,19 @@ intros l Γ A h0; split.
   + eapply TyEqRecBwd. eapply neuEq. all: try gen_typing.
     all: eapply ty_ne_term, tm_ne_conv; tea; gen_typing.
 - intros a [a' Hr Ha].
-  assert ([Γ |-[ ta ] U ≅ A]).
+  assert ([Γ |-[ ta ] U ≅ A]< wl >).
   { destruct h0; gen_typing. }
-  eapply tm_nf_conv; [| |eassumption].
+  eapply tm_nf_conv; [|eassumption].
   + eapply tm_nf_red; [eapply tmr_wf_red|]; eassumption.
-  + now eapply escape, LRU_.
 Qed.
 
-Lemma complete_ne : forall l Γ A (RA : [Γ ||-ne A]), complete (LRne_ l RA).
+Lemma complete_ne : forall l wl Γ A (RA : [Γ ||-ne A]< wl >), complete (LRne_ l RA).
 Proof.
-intros l Γ A h0; split.
+intros l wl Γ A h0; split.
 - intros ? [].
   eapply ty_nf_red; [|now apply ty_ne_nf].
   gen_typing.
-- destruct h0 as [B []]; intros ** ; assert ([Γ |- A ≅ B]) by gen_typing ; split.
+- destruct h0 as [B []]; intros ** ; assert ([Γ |- A ≅ B]< wl >) by gen_typing ; split.
   + exists n; cbn.
     * eapply redtmwf_refl ; gen_typing.
     * now eapply tm_ne_conv.
@@ -179,29 +181,44 @@ intros l Γ A h0; split.
     1,2: now eapply tm_ne_conv.
     gen_typing.
 - intros a [a' Hr Hne].
-  assert ([Γ |-[ ta ] neRedTy.ty h0 ≅ A]).
+  assert ([Γ |-[ ta ] neRedTy.ty h0 ≅ A]< wl >).
   { destruct h0; simpl in *; symmetry.
     eapply convty_exp; [now apply tyr_wf_red| |].
     all: gen_typing. }
-  eapply tm_nf_conv; [| |eassumption].
+  eapply tm_nf_conv; [|eassumption].
   + eapply tm_nf_red; [now apply tmr_wf_red|].
     now apply tm_ne_nf.
-  + now eapply escape, LRne_ with (l := l).
 Qed.
 
-Lemma complete_Pi : forall l Γ A (RA : [Γ ||-Π< l > A]),
-  (forall (Δ : context) (ρ : Δ ≤ Γ) (h : [ |-[ ta ] Δ]),
-        complete (PiRedTyPack.domRed RA ρ h)) ->
-  (forall (Δ : context) (a : term) (ρ : Δ ≤ Γ) (h : [ |-[ ta ] Δ])
-          (ha : [PiRedTyPack.domRed RA ρ h | Δ ||- a : (PiRedTyPack.dom RA)⟨ρ⟩]),
-        complete (PiRedTyPack.codRed RA ρ h ha)) ->
+Lemma complete_Pi : forall l wl Γ A (RA : [Γ ||-Π< l > A]< wl >),
+  (forall (Δ : context) (wl' : wfLCon) (ρ : Δ ≤ Γ) (τ : wl' ≤ε wl)
+          (Ninfl : (PiRedTyPack.domN RA) <= length wl')
+          (h : [ |-[ ta ] Δ]< wl' >),
+        complete (PiRedTyPack.domRed RA ρ τ Ninfl h)) ->
+  (forall (Δ : context) (a : term) (wl' : wfLCon)
+          (ρ : Δ ≤ Γ) (τ : wl' ≤ε wl)
+          (Ninfl : (PiRedTyPack.domN RA) <= length wl')
+          (h : [ |-[ ta ] Δ]< wl' >)
+          (ha : [PiRedTyPack.domRed RA ρ τ Ninfl h | Δ ||- a : (PiRedTyPack.dom RA)⟨ρ⟩]< wl' >)
+          {wl'' : wfLCon}
+          (τ' : wl'' ≤ε wl')
+          (Minfl : PiRedTyPack.codomN RA ρ τ Ninfl h ha <= length wl''),
+        complete (PiRedTyPack.codRed RA ρ τ Ninfl h ha τ' Minfl)) ->
   complete (LRPi' RA).
 Proof.
-intros l Γ A ΠA0 ihdom ihcod; split.
+  intros l wl Γ A ΠA0 ihdom ihcod.
+  split.
 - intros B ΠB.
-  assert (tΓ : [|- Γ]) by (destruct ΠA0; gen_typing).
+  assert (tΓ : [|- Γ]< wl >) by (destruct ΠA0; gen_typing).
   eapply ty_nf_red; [apply tyr_wf_red, ΠB|].
-  assert [PiRedTyPack.domRed ΠA0 wk_id tΓ | Γ ||- (PiRedTyPack.dom ΠA0)⟨wk_id⟩ ≅ PiRedTyEq.dom ΠB].
+  eapply ty_nf_prod.
+  + unshelve eapply ihdom.
+    * exact wk_id.
+    * now eapply wfLCon_le_id.
+    * 
+  assert [forall (wl' : wfLCon) (τ : wl' ≤ε wl)
+                 (Ninfl : (PiRedTyPack.domN RA) <= length wl'),
+        PiRedTyPack.domRed ΠA0 wk_id tΓ | Γ ||- (PiRedTyPack.dom ΠA0)⟨wk_id⟩ ≅ PiRedTyEq.dom ΠB]< wl >.
   1: erewrite <- wk_id_ren_on; eapply (PiRedTyEq.domRed ΠB).
   eapply ty_nf_prod.
   + now eapply ihdom.
@@ -222,8 +239,8 @@ intros l Γ A ΠA0 ihdom ihcod; split.
       * now eapply escapeConv.
 - set (ΠA := ΠA0); destruct ΠA0 as [dom cod].
   simpl in ihdom, ihcod.
-  assert [Γ |- A ≅ tProd dom cod] by gen_typing.
-  unshelve refine ( let funred : forall n, Ne[Γ |- n : A] -> [Γ |- n : A] -> [Γ |- n ~ n : A] -> [Γ ||-Π n : A | PiRedTyPack.toPiRedTy ΠA] := _ in _).
+  assert [Γ |- A ≅ tProd dom cod]< wl > by gen_typing.
+  unshelve refine ( let funred : forall n, Ne[Γ |- n : A]< wl > -> [Γ |- n : A]< wl > -> [Γ |- n ~ n : A]< wl > -> [Γ ||-Π n : A | PiRedTyPack.toPiRedTy ΠA]< wl > := _ in _).
   {
     intros. exists n; cbn.
     * eapply redtmwf_refl ; gen_typing.
@@ -276,21 +293,21 @@ intros l Γ A ΠA0 ihdom ihcod; split.
     eapply escapeEqTerm; eapply LREqTermRefl_; eassumption.
 - intros a [a' Hr Ha].
   destruct ΠA0 as [dom codom]; simpl in *.
-  assert ([Γ |- tProd dom codom ≅ A ]) by gen_typing.
+  assert ([Γ |- tProd dom codom ≅ A ]< wl >) by gen_typing.
   eapply tm_nf_conv; [| |eassumption].
   * eapply tm_nf_red; [now apply tmr_wf_red|].
     assumption.
   * destruct red; gen_typing.
 Qed.
 
-Lemma complete_Nat {l Γ A} (NA : [Γ ||-Nat A]) : complete (LRNat_ l NA).
+Lemma complete_Nat {l wl Γ A} (NA : [Γ ||-Nat A]< wl >) : complete (LRNat_ l NA).
 Proof.
   split.
   - intros ? [].
     eapply ty_nf_red, ty_nf_nat; gen_typing.
   - intros. 
-    assert [Γ |- A ≅ tNat] by (destruct NA; gen_typing). 
-    assert [Γ |- n : tNat] by now eapply ty_conv.
+    assert [Γ |- A ≅ tNat]< wl > by (destruct NA; gen_typing). 
+    assert [Γ |- n : tNat]< wl > by now eapply ty_conv.
     split; econstructor.
     1,4,5: eapply redtmwf_refl; tea; now eapply ty_conv.
     2,4: do 2 constructor; tea.
@@ -299,11 +316,11 @@ Proof.
     4-6: now (eapply tm_ne_conv; gen_typing).
     all: eapply convneu_conv; tea.
   - simpl in *.
-    assert [Γ |- tNat ≅ A] by (destruct NA; gen_typing).
-    assert [Γ |- A] by now (destruct NA; gen_typing).
+    assert [Γ |- tNat ≅ A]< wl > by (destruct NA; gen_typing).
+    assert [Γ |- A]< wl > by now (destruct NA; gen_typing).
     intros a Ha; eapply tm_nf_conv; [|eassumption|eassumption]; revert a Ha.
     let T := match goal with |- ?P => P end in
-    enough (IH : T × (forall (a : term) (n : NatProp NA a), Nf[ Γ |-[ ta ] a : tNat])); [apply IH|].
+    enough (IH : T × (forall (a : term) (n : NatProp NA a), Nf[ Γ |-[ ta ] a : tNat]< wl >)); [apply IH|].
     apply NatRedInduction.
     + intros.
       eapply tm_nf_red; [now apply tmr_wf_red|eassumption].
@@ -312,14 +329,14 @@ Proof.
     + intros ne []. apply tm_ne_nf. assumption.
 Qed.
 
-Lemma complete_Empty {l Γ A} (NA : [Γ ||-Empty A]) : complete (LREmpty_ l NA).
+Lemma complete_Empty {l wl Γ A} (NA : [Γ ||-Empty A]< wl >) : complete (LREmpty_ l NA).
 Proof.
   split.
   - intros ? [].
     eapply ty_nf_red, ty_nf_empty; gen_typing.
   - intros. 
-    assert [Γ |- A ≅ tEmpty] by (destruct NA; gen_typing). 
-    assert [Γ |- n : tEmpty] by now eapply ty_conv.
+    assert [Γ |- A ≅ tEmpty]< wl > by (destruct NA; gen_typing). 
+    assert [Γ |- n : tEmpty]< wl > by now eapply ty_conv.
     split; econstructor.
     1,4,5: eapply redtmwf_refl; tea; now eapply ty_conv.
     2,4: do 2 constructor; tea.
@@ -328,7 +345,7 @@ Proof.
     4-6: now (eapply tm_ne_conv; gen_typing).
     all: eapply convneu_conv; tea.
   - simpl in *.
-    assert [Γ |- tEmpty ≅ A] by (destruct NA; gen_typing).
+    assert [Γ |- tEmpty ≅ A]< wl > by (destruct NA; gen_typing).
     intros a Ha; eapply tm_nf_conv; [| |eassumption].
     + destruct Ha.
       destruct prop.
@@ -338,9 +355,9 @@ Proof.
     + destruct NA as [[]]; gen_typing.
 Qed.
 
-Lemma completeness {l Γ A} (RA : [Γ ||-<l> A]) : complete RA.
+Lemma completeness {l wl Γ A} (RA : [Γ ||-<l> A]< wl >) : complete RA.
 Proof.
-revert l Γ A RA; eapply LR_rect_TyUr; cbn; intros.
+revert l wl Γ A RA; eapply LR_rect_TyUr; cbn; intros.
 - now apply complete_U.
 - now apply complete_ne.
 - now apply complete_Pi.
@@ -348,38 +365,38 @@ revert l Γ A RA; eapply LR_rect_TyUr; cbn; intros.
 - now apply complete_Empty.
 Qed.
 
-Lemma neuTerm {l Γ A} (RA : [Γ ||-<l> A]) {n} :
-  Ne[Γ |- n : A] ->
-  [Γ |- n : A] ->
-  [Γ |- n ~ n : A] ->
-  [Γ ||-<l> n : A | RA].
+Lemma neuTerm {l wl Γ A} (RA : [Γ ||-<l> A]< wl >) {n} :
+  Ne[Γ |- n : A]< wl > ->
+  [Γ |- n : A]< wl > ->
+  [Γ |- n ~ n : A]< wl > ->
+  [Γ ||-<l> n : A | RA]< wl >.
 Proof.
   intros.  now eapply completeness.
 Qed.
 
-Lemma neuTermEq {l Γ A} (RA : [Γ ||-<l> A]) {n n'} :
-  Ne[Γ |- n : A] ->
-  Ne[Γ |- n' : A] ->
-  [Γ |- n : A] ->
-  [Γ |- n' : A] ->
-  [Γ |- n ~ n' : A] ->
-  [Γ ||-<l> n ≅ n' : A| RA].
+Lemma neuTermEq {l wl Γ A} (RA : [Γ ||-<l> A]< wl >) {n n'} :
+  Ne[Γ |- n : A]< wl > ->
+  Ne[Γ |- n' : A]< wl > ->
+  [Γ |- n : A]< wl > ->
+  [Γ |- n' : A]< wl > ->
+  [Γ |- n ~ n' : A]< wl > ->
+  [Γ ||-<l> n ≅ n' : A| RA]< wl >.
 Proof.
   intros; now eapply completeness.
 Qed.
 
-Lemma var0conv {l Γ A A'} (RA : [Γ ,, A ||-<l> A']) :
-  [Γ,, A |- A⟨↑⟩ ≅ A'] ->
-  [Γ |- A] ->
-  [Γ ,, A ||-<l> tRel 0 : A' | RA].
+Lemma var0conv {l wl Γ A A'} (RA : [Γ ,, A ||-<l> A']< wl >) :
+  [Γ,, A |- A⟨↑⟩ ≅ A']< wl > ->
+  [Γ |- A]< wl > ->
+  [Γ ,, A ||-<l> tRel 0 : A' | RA]< wl >.
 Proof.
   apply complete_var0 ; now eapply completeness.
 Qed.
 
-Lemma var0 {l Γ A A'} (RA : [Γ ,, A ||-<l> A']) :
+Lemma var0 {l wl Γ A A'} (RA : [Γ ,, A ||-<l> A']< wl >) :
   A⟨↑⟩ = A' ->
-  [Γ |- A] ->
-  [Γ ,, A ||-<l> tRel 0 : A' | RA].
+  [Γ |- A]< wl > ->
+  [Γ ,, A ||-<l> tRel 0 : A' | RA]< wl >.
 Proof.
   intros eq.
   apply var0conv.
@@ -388,12 +405,12 @@ Proof.
   eapply LRTyEqRefl_.
 Qed.
 
-Lemma reifyTerm {l Γ A} (RA : [Γ ||-<l> A]) {t} : [Γ ||-<l> t : A | RA] -> Nf[Γ |- t : A].
+Lemma reifyTerm {l wl Γ A} (RA : [Γ ||-<l> A]< wl >) {t} : [Γ ||-<l> t : A | RA]< wl > -> Nf[Γ |- t : A]< wl >.
 Proof.
 intros; now eapply completeness.
 Qed.
 
-Lemma reifyType {l Γ A} (RA : [Γ ||-<l> A]) : Nf[Γ |- A].
+Lemma reifyType {l wl Γ A} (RA : [Γ ||-<l> A]< wl >) : Nf[Γ |- A]< wl >.
 Proof.
   unshelve eapply reifyTyConv; tea.
   1: now eapply completeness.
