theories/LogicalRelation/Universe.v
@@ -8,21 +8,21 @@ Set Printing Universes.
 Section UniverseReducibility.
   Context `{GenericTypingProperties}.
 
-  Lemma redUOne {Γ l A} : [Γ ||-<l> A] -> [Γ ||-U<one> U].
+  Lemma redUOne {wl Γ l A} : [Γ ||-<l> A]< wl > -> [Γ ||-U<one> U]< wl >.
   Proof.
     intros ?%escape; econstructor; [easy| gen_typing|eapply redtywf_refl; gen_typing].
   Qed.
 
-  Lemma UnivEq'@{i j k l} {Γ A l} (rU : [ LogRel@{i j k l} l | Γ ||- U ]) (rA : [ LogRel@{i j k l} l | Γ ||- A : U | rU])
-    : [ LogRel@{i j k l} zero | Γ ||- A].
+  Lemma UnivEq'@{i j k l} {wl Γ A l} (rU : [ LogRel@{i j k l} l | Γ ||- U ]< wl >) (rA : [ LogRel@{i j k l} l | Γ ||- A : U | rU]< wl >)
+    : [ LogRel@{i j k l} zero | Γ ||- A]< wl >.
   Proof.
-    assert [ LogRel@{i j k l} one | Γ ||- A : U | LRU_@{i j k l} (redUOne rU)]
+    assert [ LogRel@{i j k l} one | Γ ||- A : U | LRU_@{i j k l} (redUOne rU)]< wl >
              as [ _ _ _ _ _ hA ] by irrelevance.
     exact (LRCumulative hA).
   Qed.
 
-  Lemma UnivEq@{i j k l} {Γ A l} l' (rU : [ LogRel@{i j k l} l | Γ ||- U]) (rA : [ LogRel@{i j k l} l | Γ ||- A : U | rU])
-    : [ LogRel@{i j k l} l' | Γ ||- A].
+  Lemma UnivEq@{i j k l} {wl Γ A l} l' (rU : [ LogRel@{i j k l} l | Γ ||- U]< wl >) (rA : [ LogRel@{i j k l} l | Γ ||- A : U | rU]< wl >)
+    : [ LogRel@{i j k l} l' | Γ ||- A]< wl >.
   Proof.
     destruct l'.
     - eapply (UnivEq' rU rA).
@@ -31,10 +31,10 @@ Section UniverseReducibility.
       + apply (UnivEq' rU rA).
   Qed.
 
-  Lemma UnivEqEq@{i j k l} {Γ A B l l'} (rU : [ LogRel@{i j k l} l | Γ ||- U ]) (rA : [LogRel@{i j k l} l' | Γ ||- A ]) (rAB : [ LogRel@{i j k l} l | Γ ||- A ≅ B : U | rU ])
-    : [ LogRel@{i j k l} l' | Γ ||- A ≅ B | rA ].
+  Lemma UnivEqEq@{i j k l} {wl Γ A B l l'} (rU : [ LogRel@{i j k l} l | Γ ||- U ]< wl >) (rA : [LogRel@{i j k l} l' | Γ ||- A ]< wl >) (rAB : [ LogRel@{i j k l} l | Γ ||- A ≅ B : U | rU ]< wl >)
+    : [ LogRel@{i j k l} l' | Γ ||- A ≅ B | rA ]< wl >.
   Proof.
-    assert [ LogRel@{i j k l} one | Γ ||- A ≅ B : U | LRU_@{i j k l} (redUOne rU) ] as [ _ _ _ hA _ hAB ] by irrelevance.
+    assert [ LogRel@{i j k l} one | Γ ||- A ≅ B : U | LRU_@{i j k l} (redUOne rU) ]< wl > as [ _ _ _ hA _ hAB ] by irrelevance.
     eapply LRTyEqIrrelevantCum. exact hAB.
   Qed.
 
@@ -43,25 +43,25 @@ Section UniverseReducibility.
      at the right levels for fundamental lemma ! *)
 
   Set Printing Universes.
-  Lemma univTmTy'@{h i j k l} {Γ l UU A} (h : [Γ ||-U<l> UU ]) :
-    [LogRel@{i j k l} l | Γ ||- A : UU | LRU_ h] -> [LogRel@{h i j k} (URedTy.level h) | Γ ||- A].
+  Lemma univTmTy'@{h i j k l} {wl Γ l UU A} (h : [Γ ||-U<l> UU ]< wl >) :
+    [LogRel@{i j k l} l | Γ ||- A : UU | LRU_ h]< wl > -> [LogRel@{h i j k} (URedTy.level h) | Γ ||- A]< wl >.
   Proof.  intros []; now eapply RedTyRecFwd. Qed.
 
-  Lemma univTmTy@{h i j k l} {Γ l A} (RU : [Γ ||-<l> U]) :
-    [LogRel@{i j k l} l | Γ ||- A : U | RU] -> [LogRel@{h i j k} (URedTy.level (invLRU RU)) | Γ ||- A].
+  Lemma univTmTy@{h i j k l} {wl Γ l A} (RU : [Γ ||-<l> U]< wl >) :
+    [LogRel@{i j k l} l | Γ ||- A : U | RU]< wl > -> [LogRel@{h i j k} (URedTy.level (invLRU RU)) | Γ ||- A]< wl >.
   Proof.
     intros h; apply univTmTy'.
     irrelevance.
   Qed.
 
-  Lemma univEqTmEqTy'@{h i j k l} {Γ l l' UU A B} (h : [Γ ||-U<l> UU]) (RA : [Γ ||-<l'> A]) :
-    [LogRel@{i j k l} l | Γ ||- A ≅ B : UU | LRU_ h] ->
-    [LogRel@{h i j k} l' | Γ ||- A ≅ B | RA].
+  Lemma univEqTmEqTy'@{h i j k l} {wl Γ l l' UU A B} (h : [Γ ||-U<l> UU]< wl >) (RA : [Γ ||-<l'> A]< wl >) :
+    [LogRel@{i j k l} l | Γ ||- A ≅ B : UU | LRU_ h]< wl > ->
+    [LogRel@{h i j k} l' | Γ ||- A ≅ B | RA]< wl >.
   Proof. intros [????? RA']. apply TyEqRecFwd in RA'. irrelevance. Qed.
 
-  Lemma univEqTmEqTy@{h i j k l} {Γ l l' A B} (RU : [Γ ||-<l> U]) (RA : [Γ ||-<l'> A]) :
-    [LogRel@{i j k l} l | Γ ||- A ≅ B : U | RU] ->
-    [LogRel@{h i j k} l' | Γ ||- A ≅ B | RA].
+  Lemma univEqTmEqTy@{h i j k l} {wl Γ l l' A B} (RU : [Γ ||-<l> U]< wl >) (RA : [Γ ||-<l'> A]< wl >) :
+    [LogRel@{i j k l} l | Γ ||- A ≅ B : U | RU]< wl > ->
+    [LogRel@{h i j k} l' | Γ ||- A ≅ B | RA]< wl >.
   Proof. intros h; eapply (univEqTmEqTy' (invLRU RU)); irrelevance. Qed.
 
 End UniverseReducibility.
