theories/LogicalRelation/Weakening.v
@@ -115,97 +115,114 @@ Section Weakenings.
     - intros; eapply LREmpty_; now eapply wkEmpty.
   Defined.
 
-  Definition wkΠ' {Γ Δ A l} (ρ : Δ ≤ Γ) (wfΔ : [|- Δ]) (ΠA : [Γ ||-Π< l > A]) :=
-    let ihdom Δ' (ρ' : Δ' ≤ Δ) (h : [ |- Δ']) := wk ρ' h (PiRedTyPack.domRed ΠA ρ wfΔ) in
+  Definition wkΠ' {wl Γ Δ A l} (ρ : Δ ≤ Γ) (wfΔ : [|- Δ]< wl >) (ΠA : [Γ ||-Π< l > A]< wl >) :=
+    (*let ihdom Δ' (ρ' : Δ' ≤ Δ) (h : [ |- Δ']) := wk ρ' h (PiRedTyPack.domRed ΠA ρ wfΔ) in
     let ihcod a (ha : [PiRedTyPack.domRed ΠA ρ wfΔ | _ ||- a : _]) Δ' (ρ' : Δ' ≤ Δ) (h : [ |- Δ']) :=
       wk ρ' h (PiRedTyPack.codRed ΠA ρ wfΔ ha) 
-    in
-    wkΠ ρ wfΔ ΠA ihdom ihcod.
+    in*)
+    wkΠ ΠA ρ wfΔ.
 
-  Lemma wkΠ_eq {Γ Δ A l} (ρ : Δ ≤ Γ) (wfΔ : [|- Δ]) (ΠA : [Γ ||-Π< l > A]) :
+  Lemma wkΠ_eq {wl Γ Δ A l} (ρ : Δ ≤ Γ) (wfΔ : [|- Δ]< wl >) (ΠA : [Γ ||-Π< l > A]< wl >) :
     wk ρ wfΔ (LRPi' ΠA) = LRPi' (wkΠ' ρ wfΔ ΠA).
   Proof. reflexivity. Qed.
 
   Set Printing Primitive Projection Parameters.
 
-  Lemma wkEq@{i j k l} {Γ Δ A B l} (ρ : Δ ≤ Γ) (wfΔ : [|-Δ]) (lrA : [Γ ||-<l> A]) : 
-    [LogRel@{i j k l} l | Γ ||- A ≅ B | lrA] ->
-    [LogRel@{i j k l} l | Δ ||- A⟨ρ⟩ ≅ B⟨ρ⟩ | wk ρ wfΔ lrA].
+  Lemma wkEq@{i j k l} {wl Γ Δ A B l} (ρ : Δ ≤ Γ) (wfΔ : [|-Δ]< wl >)
+    (lrA : [Γ ||-<l> A]< wl >) : 
+    [LogRel@{i j k l} l | Γ ||- A ≅ B | lrA]< wl > ->
+    [LogRel@{i j k l} l | Δ ||- A⟨ρ⟩ ≅ B⟨ρ⟩ | wk ρ wfΔ lrA]< wl >.
   Proof.
-    revert B Δ ρ wfΔ. pattern l, Γ, A, lrA.
-    eapply LR_rect_TyUr; clear l Γ A lrA.
-    - intros ?? ????? ? [] ; constructor; change U with U⟨ρ⟩; gen_typing.
+    revert B Δ ρ wfΔ. pattern l, wl, Γ, A, lrA.
+    eapply LR_rect_TyUr; clear l wl Γ A lrA.
+    - intros ??? ????? ? [] ; constructor; change U with U⟨ρ⟩; gen_typing.
     - intros * [ty].
       exists ty⟨ρ⟩.
       2: now apply ty_ne_wk, ne.
       1: gen_typing.
       cbn ; change U with U⟨ρ⟩; eapply convneu_wk; assumption.
     - intros * ihdom ihcod * [dom cod]. rewrite wkΠ_eq. set (X := wkΠ' _ _ _).
-      exists (dom⟨ρ⟩) (cod⟨wk_up dom ρ⟩). cbn in *.
+      unshelve econstructor.
+      + exact (dom⟨ρ⟩).
+      + exact (cod⟨wk_up dom ρ⟩).
+      + exact domN.
+      + unfold wkΠ'. intros ; unshelve eapply (codomN Δ0 a l' (ρ0 ∘w ρ) τ Ninfl Ninfl' h).
+        subst X.
+        irrelevance.
       + change (tProd _ _) with ((tProd dom cod)⟨ρ⟩);  gen_typing.
       + change (tProd dom⟨_⟩ _) with ((tProd dom cod)⟨ρ⟩).
         replace (tProd _ _) with ((PiRedTyPack.prod ΠA)⟨ρ⟩) by now bsimpl.
         eapply convty_wk; assumption.
       + intros; irrelevanceRefl.
-        unshelve eapply ihdom; try eassumption; eapply domRed.
-      + intros ? a ρ' ??.
+        unshelve eapply ihdom; try eassumption.
+        * now eapply wfc_Ltrans.
+        * now eapply domRed.
+      + intros ? a wl' ρ' ?????????.
         replace (_[_ .: ρ' >> tRel]) with (cod[ a .: (ρ' ∘w ρ) >> tRel]) by now bsimpl.
         irrelevance0.
-        2: unshelve eapply codRed; [eassumption|]; subst X; irrelevance.
+        2: unshelve eapply codRed ; [exact wl'|..] ; subst X ; try irrelevance ; assumption.
         subst X; bsimpl; try rewrite scons_comp'; reflexivity.
     - intros * []; constructor.
       change tNat with tNat⟨ρ⟩; gen_typing.
+    - intros * []; constructor.
+      change tBool with tBool⟨ρ⟩; gen_typing.
     - intros * []; constructor.
       change tEmpty with tEmpty⟨ρ⟩; gen_typing.
   Qed.
     
 
   (* TODO: use program or equivalent to have only the first field non-opaque *)
-  Lemma wkΠTerm {Γ Δ u A l} (ρ : Δ ≤ Γ) (wfΔ : [|- Δ]) (ΠA : [Γ ||-Π< l > A]) 
+  Lemma wkΠTerm {wl Γ Δ u A l} (ρ : Δ ≤ Γ) (wfΔ : [|- Δ]< wl >) (ΠA : [Γ ||-Π< l > A]< wl >) 
     (ΠA' := wkΠ' ρ wfΔ ΠA) : 
-    [Γ||-Π u : A | PiRedTyPack.toPiRedTy ΠA] -> 
-    [Δ ||-Π u⟨ρ⟩ : A⟨ρ⟩ | PiRedTyPack.toPiRedTy ΠA' ].
+    [Γ||-Π u : A | PiRedTyPack.toPiRedTy ΠA]< wl > -> 
+    [Δ ||-Π u⟨ρ⟩ : A⟨ρ⟩ | PiRedTyPack.toPiRedTy ΠA' ]< wl >.
   Proof.
-    intros [t].
-    exists (t⟨ρ⟩); try change (tProd _ _) with ((PiRedTyPack.prod ΠA)⟨ρ⟩).
-    + now eapply redtmwf_wk.
-    + apply isFun_ren; assumption.
-    + now apply tm_nf_wk.
-    + eapply convtm_wk; eassumption.
-    + intros ? a ρ' ??.
+    intros [t]. 
+    unshelve econstructor ;  try change (tProd _ _) with ((PiRedTyPack.prod ΠA)⟨ρ⟩).
+    - exact (t⟨ρ⟩).
+    - exact redN.
+    - intros ; unshelve eapply appN ; try assumption.
+      exact (ρ0 ∘w ρ).
+      subst ΠA'. 
+      irrelevance.
+    - now eapply redtmwf_wk.
+    - apply isFun_ren; assumption.
+    - now apply tm_nf_wk.
+    - eapply convtm_wk; eassumption.
+    - intros ? a ? ρ' * ?.
       replace ((t ⟨ρ⟩)⟨ ρ' ⟩) with (t⟨ρ' ∘w ρ⟩) by now bsimpl.
       irrelevance0.
-      2: unshelve apply app; [eassumption|]; subst ΠA'; irrelevance. 
+      2: unshelve eapply app;  [exact l'|..]; subst ΠA'; try irrelevance ; assumption. 
       subst ΠA'; bsimpl; try rewrite scons_comp'; reflexivity.
-    + intros ??? ρ' ????.
+    - intros ???? ρ' ???????????.
       replace ((t ⟨ρ⟩)⟨ ρ' ⟩) with (t⟨ρ' ∘w ρ⟩) by now bsimpl.
       irrelevance0.
-      2: unshelve apply eq; [eassumption|..]; subst ΠA'; irrelevance.
+      2: unshelve eapply eq;  [exact l'|..]; subst ΠA'; try irrelevance ; assumption.
       subst ΠA'; bsimpl; try rewrite scons_comp'; reflexivity.
   Defined.
 
-  Lemma wkNeNf {Γ Δ k A} (ρ : Δ ≤ Γ) (wfΔ : [|-Δ]) : 
-    [Γ ||-NeNf k : A] -> [Δ ||-NeNf k⟨ρ⟩ : A⟨ρ⟩].
+  Lemma wkNeNf {wl Γ Δ k A} (ρ : Δ ≤ Γ) (wfΔ : [|-Δ]< wl >) : 
+    [Γ ||-NeNf k : A]< wl > -> [Δ ||-NeNf k⟨ρ⟩ : A⟨ρ⟩]< wl >.
   Proof.
     intros []; constructor. 1:apply tm_ne_wk. all: gen_typing.
   Qed.  
 
-  Lemma wkTerm {Γ Δ t A l} (ρ : Δ ≤ Γ) (wfΔ : [|-Δ]) (lrA : [Γ ||-<l> A]) : 
-    [Γ ||-<l> t : A | lrA] -> [Δ ||-<l> t⟨ρ⟩ : A⟨ρ⟩ | wk ρ wfΔ lrA].
+  Lemma wkTerm {wl Γ Δ t A l} (ρ : Δ ≤ Γ) (wfΔ : [|-Δ]< wl >) (lrA : [Γ ||-<l> A]< wl >) : 
+    [Γ ||-<l> t : A | lrA]< wl > -> [Δ ||-<l> t⟨ρ⟩ : A⟨ρ⟩ | wk ρ wfΔ lrA]< wl >.
   Proof.
-    revert t Δ ρ wfΔ. pattern l, Γ, A, lrA.
-    eapply LR_rect_TyUr; clear l Γ A lrA.
-    - intros ?????? ρ ? [te]; exists te⟨ρ⟩;  try change U with U⟨ρ⟩.
+    revert t Δ ρ wfΔ. pattern l, wl, Γ, A, lrA.
+    eapply LR_rect_TyUr; clear l wl Γ A lrA.
+    - intros ??????? ρ ? [te]; exists te⟨ρ⟩;  try change U with U⟨ρ⟩.
       1, 4: gen_typing.
       apply isType_ren; assumption.
       now apply tm_nf_wk.
       apply RedTyRecBwd ; apply wk; [assumption|]; now apply (RedTyRecFwd h).
-    - intros ?????? ρ ? [te]. exists te⟨ρ⟩; cbn.
+    - intros ??????? ρ ? [te]. exists te⟨ρ⟩; cbn.
       + now eapply redtmwf_wk.
       + apply tm_ne_wk; assumption.
       + eapply convneu_wk; eassumption.
-    - intros ???? ihdom ihcod ?? ρ ?; apply wkΠTerm. 
-    - intros??? NA t ? ρ wfΔ; revert t; pose (NA' := wkNat ρ wfΔ NA).
+    - intros ????? ihdom ihcod ?? ρ ?; apply wkΠTerm. 
+    - intros ???? NA t ? ρ wfΔ; revert t; pose (NA' := wkNat ρ wfΔ NA).
       set (G := _); enough (h : G × (forall t, NatProp NA t -> NatProp NA' t⟨ρ⟩)) by apply h.
       subst G; apply NatRedInduction.
       + intros; econstructor; tea; change tNat with tNat⟨ρ⟩; gen_typing.
@@ -214,23 +231,26 @@ Section Weakenings.
       + intros; constructor. 
         change tNat with tNat⟨ρ⟩.
         now eapply wkNeNf.
-    - intros??? NA t ? ρ wfΔ; revert t; pose (NA' := wkEmpty ρ wfΔ NA).
-      set (G := _); enough (h : G × (forall t, EmptyProp Γ t -> EmptyProp Δ t⟨ρ⟩)) by apply h.
-      subst G.
-      split.
-      2:{ intros t Ht. inversion Ht. subst. econstructor.
-          change tEmpty with tEmpty⟨ρ⟩.
-          now eapply wkNeNf. }
-      intros t Ht. induction Ht. econstructor.
+    - intros ???? NA t ? ρ wfΔ.
+      intros Ht ; induction Ht.
+      econstructor.
+      + change tBool with tBool⟨ρ⟩. gen_typing.
+      + change tBool with tBool⟨ρ⟩. gen_typing.
+      + clear red eq. inversion prop ; subst ; try now econstructor.
+          constructor.
+          change tBool with tBool⟨ρ⟩.
+          now eapply wkNeNf.
+    - intros ???? NA t ? ρ wfΔ.
+      intro Ht ; induction Ht ; econstructor.
       + change tEmpty with tEmpty⟨ρ⟩; gen_typing.
       + change tEmpty with tEmpty⟨ρ⟩; gen_typing.
-      + destruct prop. econstructor.
+      + inversion prop ; subst ; econstructor.
         change tEmpty with tEmpty⟨ρ⟩.
         now eapply wkNeNf.
   Qed.
 
-  Lemma wkUTerm {Γ Δ l A t} (ρ : Δ ≤ Γ) (wfΔ : [|-Δ]) (h : [Γ ||-U<l> A]) :
-    [LogRelRec l| Γ ||-U t : A | h ] -> [LogRelRec l | Δ||-U t⟨ρ⟩ : A⟨ρ⟩ | wkU ρ wfΔ h].
+  Lemma wkUTerm {wl Γ Δ l A t} (ρ : Δ ≤ Γ) (wfΔ : [|-Δ]< wl >) (h : [Γ ||-U<l> A]< wl >) :
+    [LogRelRec l| Γ ||-U t : A | h ]< wl > -> [LogRelRec l | Δ||-U t⟨ρ⟩ : A⟨ρ⟩ | wkU ρ wfΔ h]< wl >.
   Proof.
     intros [te]. exists te⟨ρ⟩; change U with U⟨ρ⟩.
     1, 4: gen_typing.
@@ -240,18 +260,18 @@ Section Weakenings.
     eapply (wk (l:=zero)); eassumption.
   Defined.
 
-  Lemma wkNeNfEq {Γ Δ k k' A} (ρ : Δ ≤ Γ) (wfΔ : [|-Δ]) : 
-    [Γ ||-NeNf k ≅ k' : A] -> [Δ ||-NeNf k⟨ρ⟩ ≅ k'⟨ρ⟩ : A⟨ρ⟩].
+  Lemma wkNeNfEq {wl Γ Δ k k' A} (ρ : Δ ≤ Γ) (wfΔ : [|-Δ]< wl >) : 
+    [Γ ||-NeNf k ≅ k' : A]< wl > -> [Δ ||-NeNf k⟨ρ⟩ ≅ k'⟨ρ⟩ : A⟨ρ⟩]< wl >.
   Proof.
     intros []; constructor. 1,2: apply tm_ne_wk. all: gen_typing.
   Qed.  
 
-  Lemma wkTermEq {Γ Δ t u A l} (ρ : Δ ≤ Γ) (wfΔ : [|-Δ]) (lrA : [Γ ||-<l> A]) : 
-    [Γ ||-<l> t ≅ u : A | lrA] -> [Δ ||-<l> t⟨ρ⟩ ≅ u⟨ρ⟩: A⟨ρ⟩ | wk ρ wfΔ lrA].
+  Lemma wkTermEq {wl Γ Δ t u A l} (ρ : Δ ≤ Γ) (wfΔ : [|-Δ]< wl >) (lrA : [Γ ||-<l> A]< wl >) : 
+    [Γ ||-<l> t ≅ u : A | lrA]< wl > -> [Δ ||-<l> t⟨ρ⟩ ≅ u⟨ρ⟩: A⟨ρ⟩ | wk ρ wfΔ lrA]< wl >.
   Proof.
-    revert t u Δ ρ wfΔ. pattern l, Γ, A, lrA.
-    eapply LR_rect_TyUr; clear l Γ A lrA.
-    - intros ??????? ρ ? [rL rR].
+    revert t u Δ ρ wfΔ. pattern l, wl, Γ, A, lrA.
+    eapply LR_rect_TyUr; clear l wl Γ A lrA.
+    - intros ???????? ρ ? [rL rR].
       unshelve econstructor.
       + exact (wkUTerm ρ wfΔ h rL).
       + exact (wkUTerm ρ wfΔ h rR).
@@ -260,23 +280,27 @@ Section Weakenings.
         now eapply convtm_wk.
       + apply RedTyRecBwd; apply wk; [assumption|]; now apply (RedTyRecFwd h).
       + apply TyEqRecBwd. eapply wkEq. now apply TyEqRecFwd.
-    - intros ??????? ρ ? [tL tR].
+    - intros ???????? ρ ? [tL tR].
       exists (tL⟨ρ⟩) (tR⟨ρ⟩); cbn.
       1,2: now eapply redtmwf_wk. 
       1,2: apply tm_ne_wk; assumption.
       now eapply convneu_wk.
-    - intros ??? ΠA ihdom ihcod t u ? ρ ? [redL redR].
+    - intros ???? ΠA ihdom ihcod t u ? ρ ? [redL redR].
       rewrite wkΠ_eq. set (X := wkΠ' _ _).
       unshelve econstructor; try change (tProd _ _) with ((PiRedTyPack.prod ΠA)⟨ρ⟩).
       1,2: now eapply wkΠTerm.
+      + assumption.
+      + intros ; unshelve eapply eqappN ; try assumption.
+        exact (ρ0 ∘w ρ).
+        subst X. 
+        irrelevance.
       + now eapply convtm_wk.
-      + intros ? a ρ' ? ?. 
+      + intros ? a ? ρ' * ?. 
         replace (_ ⟨ ρ' ⟩) with (PiRedTm.nf redL) ⟨ρ' ∘w ρ⟩ by now bsimpl.
         replace (_ ⟨ ρ' ⟩) with (PiRedTm.nf redR) ⟨ρ' ∘w ρ⟩ by now bsimpl.
-        irrelevance0.  2: unshelve eapply eqApp; [assumption|].
-        2: irrelevance; subst X; now bsimpl.
+        irrelevance0.  2: unshelve eapply eqApp; [exact l'|..]; subst X; try irrelevance ; assumption. 
         subst X; bsimpl; now try rewrite scons_comp'.
-    - intros??? NA t u ? ρ wfΔ; revert t u; pose (NA' := wkNat ρ wfΔ NA).
+    - intros ???? NA t u ? ρ wfΔ; revert t u; pose (NA' := wkNat ρ wfΔ NA).
       set (G := _); enough (h : G × (forall t u, NatPropEq NA t u -> NatPropEq NA' t⟨ρ⟩ u⟨ρ⟩)) by apply h.
       subst G; apply NatRedEqInduction.
       + intros; econstructor; tea; change tNat with tNat⟨ρ⟩; gen_typing.
@@ -285,17 +309,20 @@ Section Weakenings.
       + intros; constructor. 
         change tNat with tNat⟨ρ⟩.
         now eapply wkNeNfEq.
-    - intros??? NA t u ? ρ wfΔ; revert t u; pose (NA' := wkEmpty ρ wfΔ NA).
-      set (G := _); enough (h : G × (forall t u, EmptyPropEq Γ t u -> EmptyPropEq Δ t⟨ρ⟩ u⟨ρ⟩)) by apply h.
-      subst G. split.
-      2:{ intros t u Ht. inversion Ht. subst. econstructor.
-          change tEmpty with tEmpty⟨ρ⟩.
-          now eapply wkNeNfEq. }
-      intros t u Ht. induction Ht. econstructor.
+    - intros ???? NA t u ? ρ wfΔ Ht.
+      induction Ht ; econstructor.
+      + change tBool with tBool⟨ρ⟩; gen_typing.
+      + change tBool with tBool⟨ρ⟩; gen_typing.
+      + change tBool with tBool⟨ρ⟩; gen_typing.
+      + inversion prop ; subst ; econstructor.
+        change tBool with tBool⟨ρ⟩.
+          now eapply wkNeNfEq.
+    - intros ???? NA t u ? ρ wfΔ Ht.
+      induction Ht ; econstructor.
       + change tEmpty with tEmpty⟨ρ⟩; gen_typing.
       + change tEmpty with tEmpty⟨ρ⟩; gen_typing.
       + change tEmpty with tEmpty⟨ρ⟩; gen_typing.
-      + destruct prop. econstructor.
+      + inversion prop ; subst ; econstructor.
         change tEmpty with tEmpty⟨ρ⟩.
         now eapply wkNeNfEq.
   Qed.
